MPL/SpecAttr.lean
@@ -1,136 +1,112 @@
 /-
 Copyright (c) 2025 Lean FRO LLC. All rights reserved.
 Released under Apache 2.0 license as described in the file LICENSE.
-Authors: Son Ho, Sebastian Graf
+Authors: Sebastian Graf
 -/
 import Lean
 import MPL.Triple
-
--- This file is based on
--- https://github.com/AeneasVerif/aeneas/blob/6ff714176180068bd3873af759d26a7053f4a795/backends/lean/Aeneas/Progress/Init.lean
+import MPL.Util.Trace
 
 namespace MPL
 
 open Lean Meta
 
-/- Discrimination trees map expressions to values. When storing an expression
-   in a discrimination tree, the expression is first converted to an array
-   of `DiscrTree.Key`, which are the keys actually used by the discrimination
-   trees. The conversion operation is monadic, however, and extensions require
-   all the operations to be pure. For this reason, in the state extension, we
-   store the keys from *after* the transformation (i.e., the `DiscrTreeKey`
-   below). The transformation itself can be done elsewhere.
- -/
-abbrev DiscrTreeKey := Array DiscrTree.Key
-
-abbrev DiscrTreeExtension (α : Type) :=
-  SimplePersistentEnvExtension (DiscrTreeKey × α) (DiscrTree α)
-
-def mkDiscrTreeExtension [Inhabited α] [BEq α] (name : Name := by exact decl_name%) :
-  IO (DiscrTreeExtension α) :=
-  registerSimplePersistentEnvExtension {
-    name          := name,
-    addImportedFn := fun a => a.foldl (fun s a => a.foldl (fun s (k, v) => s.insertCore k v) s) DiscrTree.empty,
-    addEntryFn    := fun s n => s.insertCore n.1 n.2 ,
-  }
-
--- TODO SpecInfo is currently dead because we simply do the inference in `mSpec`
-structure SpecInfo where
-  /-- whether the precondition is schematic, i.e., ∀-bound variable. -/
-  preSchematic : Bool
-  /-- whether the postcondition is schematic, i.e., ∀-bound variable. -/
-  postSchematic : Bool
-  deriving Inhabited, BEq
-
-def mkSpecKeyAndInfo (ty : Expr) : MetaM (Expr × SpecInfo) := do
-  let (xs, _bis, body) ← forallMetaTelescope ty
-  let_expr Triple _m _ps _inst _α prog P Q := body | throwError s!"not a triple: {body}"
-  let f := prog.getAppFn'
-  unless f.isConst do throwError s!"not an application of a constant: {prog}"
-  let preSchematic := P.isMVar && xs.contains P
-  let postSchematic := Q.isMVar && xs.contains Q
-  return (prog, { preSchematic, postSchematic })
-
--- spec attribute
-structure SpecAttr where
-  attr : AttributeImpl
-  ext  : DiscrTreeExtension (ConstantVal × SpecInfo)
-  deriving Inhabited
-
-/-- For the attributes
-
-    If we apply an attribute to a definition in a group of mutually recursive definitions
-    (say, to `foo` in the group [`foo`, `bar`]), the attribute gets applied to `foo` but also to
-    the recursive definition which encodes `foo` and `bar` (Lean encodes mutually recursive
-    definitions in one recursive definition, e.g., `foo._mutual`, before deriving the individual
-    definitions, e.g., `foo` and `bar`, from this one). This definition should be named `foo._mutual`
-    or `bar._mutual`, and we generally want to ignore it.
-
-    TODO: same problem happens if we use decreases clauses, etc.
-
-    Below, we implement a small utility to do so.
-  -/
-def attrIgnoreAuxDef (name : Name) (default : AttrM α) (x : AttrM α) : AttrM α := do
-  -- TODO: this is a hack
-  if let .str _ "_mutual" := name then
---    trace[Utils] "Ignoring a mutually recursive definition: {name}"
-    default
-  else if let .str _ "_unary" := name then
---    trace[Utils] "Ignoring a unary def: {name}"
-    default
-  else
-    -- Normal execution
-    x
-
-initialize registerTraceClass `mpl (inherited := true)
 initialize registerTraceClass `mpl.spec.attr (inherited := true)
 
-/- The persistent map from expressions to pspec theorems. -/
-initialize specAttr : SpecAttr ← do
-  let ext ← mkDiscrTreeExtension `specMap
-  let attrImpl : AttributeImpl := {
-    name := `spec
-    descr := "Marks theorems to use with the `mspec` tactic"
-    add := fun thName stx attrKind => do
-      Attribute.Builtin.ensureNoArgs stx
-      -- TODO: use the attribute kind
-      unless attrKind == AttributeKind.global do
-        throwError "invalid attribute 'spec', must be global"
-      -- Lookup the theorem
-      let env ← getEnv
-      -- Ignore some auxiliary definitions (see the comments for attrIgnoreMutRec)
-      attrIgnoreAuxDef thName (pure ()) do
-        trace[mpl.spec.attr] "Registering spec theorem for {thName}"
-        let thDecl := env.constants.find! thName
-        let (fKey, specInfo) ← MetaM.run' do
-          let mut ty := thDecl.type
-          trace[mpl.spec.attr] "Theorem: {ty}"
-          -- Normalize to eliminate the let-bindings
---          ty ← zetaReduce ty
---          trace[mpl] "Theorem after normalization (to eliminate the let bindings): {ty}"
-          let (fExpr, specInfo) ← mkSpecKeyAndInfo ty
-          trace[mpl.spec.attr] "Registering spec theorem for expr: {fExpr}"
-          -- Convert the function expression to a discrimination tree key
-          return (← DiscrTree.mkPath fExpr, specInfo)
-        let env := ext.addEntry env (fKey, (thDecl.toConstantVal, specInfo))
-        setEnv env
-        trace[mpl.spec.attr] "Saved the environment"
-        pure ()
+structure SpecTheorem where
+  keys : Array DiscrTree.Key
+  proof : Name -- TODO: Could be Expr, as for `SimpTheorem`
+  priority : Nat  := eval_prio default -- TODO: unused
+  origin : Origin
+  /-- `rfl` is true if `proof` is by `SPred.entails.rfl`. -/
+  rfl : Bool
+  deriving Inhabited, BEq
+
+abbrev SpecEntry := SpecTheorem
+
+structure SpecTheorems where
+  specs : DiscrTree SpecTheorem := DiscrTree.empty
+  deriving Inhabited
+
+abbrev SpecExtension := SimpleScopedEnvExtension SpecEntry SpecTheorems
+
+private def mkSpecTheorem (origin : Origin) (type : Expr) (proof : Name) (prio : Nat) : MetaM SpecTheorem := do
+  -- cf. mkSimpTheoremCore
+  let type ← instantiateMVars type
+  withNewMCtxDepth do
+  let (_, _, type) ← forallMetaTelescopeReducing type
+  let type ← whnfR type
+  let_expr Triple _m _ps _inst _α prog _P _Q := type
+    | throwError "unexpected kind of spec theorem; not a triple{indentExpr type}"
+  let f := prog.getAppFn'
+  unless f.isConst do throwError s!"not an application of a constant: {prog}"
+  let keys ← DiscrTree.mkPath prog (noIndexAtArgs := false)
+  return { keys, proof, origin, rfl := false, priority := prio }
+
+private def mkSpecTheoremFromConst (declName : Name) (prio : Nat) : MetaM SpecTheorem := do
+  -- cf. mkSimpTheoremsFromConst
+  let cinfo ← getConstInfo declName
+  let us := cinfo.levelParams.map mkLevelParam
+  let origin := Origin.decl declName
+  let val := mkConst declName us
+  withSimpGlobalConfig do -- sounds like a good default here,
+    let type ← inferType val
+    unless (← isProp type) do
+      throwError "invalid 'spec', proposition expected{indentExpr type}"
+    mkSpecTheorem origin type declName prio
+
+def addSpecTheorem (ext : SpecExtension) (declName : Name) (prio : Nat) (attrKind : AttributeKind) : MetaM Unit := do
+  ext.add (← mkSpecTheoremFromConst declName prio) attrKind
+
+def addSpecTheoremEntry (d : SpecTheorems) (e : SpecTheorem) : SpecTheorems :=
+  { d with specs := d.specs.insertCore e.keys e }
+
+def mkSpecExt : IO SpecExtension :=
+  registerSimpleScopedEnvExtension {
+    name     := `specMap
+    initial  := {}
+    addEntry := addSpecTheoremEntry
   }
-  registerBuiltinAttribute attrImpl
-  pure { attr := attrImpl, ext := ext }
 
-def SpecAttr.find? (s : SpecAttr) (e : Expr) : MetaM (Array (ConstantVal × SpecInfo)) := do
-  (s.ext.getState (← getEnv)).getMatch e
+def mkSpecAttr (ext : SpecExtension) : IO Unit :=
+  registerBuiltinAttribute {
+    name  := `spec
+    descr := "Marks theorems to use with the `mspec` and `mvcgen` tactics"
+    -- applicationTime := AttributeApplicationTime.afterCompilation -- this seems unnecessarily conservative?
+    applicationTime := AttributeApplicationTime.afterTypeChecking
+    add   := fun declName stx attrKind => do
+      let go : MetaM Unit := do
+        let info ← getConstInfo declName
+        let prio ← Attribute.Builtin.getPrio stx
+        if (← isProp info.type) then
+          addSpecTheorem ext declName prio attrKind
+        -- TODO: add unfold rules
+        -- else if info.hasValue then
+        --   if (← SimpTheorems.ignoreEquations declName) then
+        --     ext.add (SimpEntry.toUnfold declName) attrKind
+        --   else if let some eqns ← getEqnsFor? declName then
+        --     for eqn in eqns do
+        --       addSimpTheorem ext eqn post (inv := false) attrKind prio
+        --     ext.add (SimpEntry.toUnfoldThms declName eqns) attrKind
+        --     if (← SimpTheorems.unfoldEvenWithEqns declName) then
+        --       ext.add (SimpEntry.toUnfold declName) attrKind
+        --   else
+        --     ext.add (SimpEntry.toUnfold declName) attrKind
+        else
+          throwError "invalid 'spec', it is not a proposition" -- nor a definition (to unfold)"
+      discard <| go.run {} {}
+      -- TODO: add erase
+  }
 
-def SpecAttr.getState (s : SpecAttr) : MetaM (DiscrTree (ConstantVal × SpecInfo)) := do
-  pure (s.ext.getState (← getEnv))
+initialize specAttr : SpecExtension ← do
+  let ext ← mkSpecExt
+  mkSpecAttr ext
+  return ext
 
-def showStoredSpec : MetaM Unit := do
-  let st ← specAttr.getState
-  -- TODO: how can we iterate over (at least) the values stored in the tree?
-  --let s := st.toList.foldl (fun s (f, th) => f!"{s}\n{f} → {th}") f!""
-  let s := f!"{st.mapArrays fun arr => arr.map (·.fst.name)}"
-  IO.println s
+def SpecExtension.getTheorems (ext : SpecExtension) : CoreM SpecTheorems :=
+  return ext.getState (← getEnv)
+
+def getSpecTheorems : CoreM SpecTheorems :=
+  specAttr.getTheorems
 
 end MPL
