MPL/Util/Trace.lean
@@ -1,0 +1,5 @@
+import Lean
+
+namespace MPL.Util
+
+initialize Lean.registerTraceClass `mpl (inherited := true)
