Test/Code.lean
@@ -1,0 +1,36 @@
+import MPL.Idd
+
+namespace MPL.Test.Code
+
+def fib_impl (n : Nat) : Idd Nat := do
+  if n = 0 then return 0
+  let mut a := 0
+  let mut b := 1
+  for _ in [1:n] do
+    let a' := a
+    a := b
+    b := a' + b
+  return b
+
+abbrev fib_spec : Nat → Nat
+| 0 => 0
+| 1 => 1
+| n+2 => fib_spec n + fib_spec (n+1)
+
+def ifs (n : Nat) : Idd Nat := do
+  let mut x := 0
+  if n > 0 then x := x + 1 else x := x + 2
+  if n > 1 then x := x + 1 else x := x + 2
+  return x
+
+abbrev AppState := Nat × Nat
+
+def mkFreshNat [Monad m] [MonadStateOf AppState m] : m Nat := do
+  let n ← Prod.fst <$> get
+  modify (fun s => (s.1 + 1, s.2))
+  pure n
+
+def mkFreshPair : StateM AppState (Nat × Nat) := do
+  let a ← mkFreshNat
+  let b ← mkFreshNat
+  pure (a, b)
